theories/DeepTyping.v
@@ -1,7 +1,7 @@
 (** * LogRel.DeclarativeInstance: proof that declarative typing is an instance of generic typing. *)
 From Coq Require Import CRelationClasses.
 From LogRel.AutoSubst Require Import core unscoped Ast Extra.
-From LogRel Require Import Utils BasicAst Notations Context Closed NormalForms UntypedReduction Weakening NormalEq GenericTyping DeclarativeTyping DeclarativeInstance.
+From LogRel Require Import Utils BasicAst Computation Notations Context Closed NormalForms UntypedReduction Weakening NormalEq GenericTyping DeclarativeTyping DeclarativeInstance.
 
 Import DeclarativeTypingData.
 
@@ -216,6 +216,20 @@ split.
       repeat rewrite <- (wk1_ren_on Γ A).
       eapply typing_wk; tea.
     * do 2 rewrite eq0; apply TermRefl; tea.
+Qed.
+
+Lemma NfTermDecl_tLambda0 : forall Γ A A₀ B t t₀,
+  [Γ |-[ de ] A] ->
+  NfTypeDecl Γ A A₀ ->
+  NfTermDecl (Γ,, A) B t t₀ ->
+  NfTermDecl Γ (tProd A B) (tLambda A t) (tLambda A₀ t₀).
+Proof.
+intros * ? [] [].
+split.
++ apply dredalg_lambda; tea.
++ now constructor.
++ constructor; tea.
+  now apply TypeRefl.
 Qed.
 
 Lemma NfTypeDecl_tSig : forall Γ A A' A₀ B B₀,
@@ -545,6 +559,34 @@ split.
   replace n₀ with n by now eapply dred_dnf.
   assumption.
 + now constructor.
+Qed.
+
+Lemma NeTermDecl_tReflect : forall Γ (t t' t₀ u u' u₀ : term),
+  [Γ |-[ de ] t ≅ t' : arr tNat tNat] ->
+  [Γ |-[ de ] u ≅ u' : tNat] ->
+  [Γ |-[ de ] model.(run) : arr tNat (arr tNat tPNat) ] ->
+  (~ closed0 t') + (~ closed0 u') -> dnf t' -> dnf u' ->
+  NfTermDecl Γ (arr tNat tNat) t' t₀ ->
+  NfTermDecl Γ tNat u' u₀ ->
+  NeTermDecl Γ (tTotal t u) (tReflect t' u') (tReflect t₀ u₀).
+Proof.
+intros * Ht Hu ? ? ? ? [] [].
+assert (t' = t₀) by now eapply dred_dnf.
+assert (u' = u₀) by now eapply dred_dnf.
+subst.
+split; [now constructor|]; split.
++ apply gred_red, redalg_reflect; tea.
++ do 2 constructor; tea.
++ eapply TermConv; [apply TermReflectCong; tea|].
+  apply convty_term, tTotal_cong.
+  - change (arr tNat tNat) with (arr tNat tNat)[u₀..].
+    eapply (TermAppCong (A := tNat)); [|now apply TermSym].
+    change (tProd tNat (arr tNat tNat)) with (arr tNat (arr tNat tNat))[(tQuote t₀)..].
+    eapply (TermAppCong (A := tNat)); [|now apply TermSym, TermQuoteCong].
+    now apply TermRefl.
+  - change tNat with tNat[u₀..].
+    eapply (TermAppCong (A := tNat)); [|now apply TermSym].
+    now apply TermSym.
 Qed.
 
 End Nf.
@@ -881,6 +923,11 @@ Module DeepTypingProperties.
     - eapply NfTermDecl_tSig; tea.
       * now eapply urefl.
     - now apply eqnf_tSig.
+  + intros; invnf; eexists.
+    - constructor; tea; now eapply TypeRefl.
+    - apply NfTermDecl_tLambda0; tea.
+    - apply NfTermDecl_tLambda0; tea.
+    - now apply eqnf_tLambda.
   + intros * ? ? ? Hf ? Hg [].
     eapply isWfFun_isNfFun in Hf; [|tea].
     eapply isWfFun_isNfFun in Hg; [|tea].
@@ -951,6 +998,7 @@ Module DeepTypingProperties.
   Proof.
   all: try apply DeclarativeTypingProperties.TypingDeclProperties.
   + intros * []; now constructor.
+  + intros * [] []; now econstructor.
   + intros * ? []; now econstructor.
   Qed.
 
@@ -1026,6 +1074,25 @@ Module DeepTypingProperties.
         replace u with n' in * by eauto using dred_dnf, nftmdecl_red, nftmdecl_nf
       end.
       now apply eqnf_tQuote.
+  + intros; invnf; eexists.
+    - now eapply convneu_reflect.
+    - apply NeTermDecl_tReflect; tea; try now eapply lrefl.
+      all: try now symmetry.
+    - apply NeTermDecl_tReflect; tea.
+      all: etransitivity; [now symmetry|tea].
+    - match goal with |- eqnf (tReflect ?f ?n) (tReflect ?g ?m) =>
+        replace f with t in * by eauto using dred_dnf, nftmdecl_red, nftmdecl_nf;
+        replace g with t' in * by eauto using dred_dnf, nftmdecl_red, nftmdecl_nf;
+        replace n with u in * by eauto using dred_dnf, nftmdecl_red, nftmdecl_nf;
+        replace m with u' in * by eauto using dred_dnf, nftmdecl_red, nftmdecl_nf
+      end.
+      match goal with H : NfTermDecl _ _  t ?r |- _ =>
+        tryif unify t r then fail else assert (r = t) by (now eapply NfTermDecl_unique); subst
+      end.
+      match goal with H : NfTermDecl _ _  u ?r |- _ =>
+        tryif unify u r then fail else assert (r = u) by (now eapply NfTermDecl_unique); subst
+      end.
+      now apply eqnf_tReflect.
   Qed.
 
   #[export, refine] Instance RedTypeDeclProperties : RedTypeProperties (ta := nf) := {}.
@@ -1038,6 +1105,8 @@ Module DeepTypingProperties.
   all: try apply DeclarativeTypingProperties.RedTermDeclProperties.
   + intros; invnf; now apply DeclarativeTypingProperties.RedTermDeclProperties.
   + intros; invnf; now apply DeclarativeTypingProperties.RedTermDeclProperties.
+  + intros; invnf; now apply DeclarativeTypingProperties.RedTermDeclProperties.
+  + intros; invnf; now eapply DeclarativeTypingProperties.RedTermDeclProperties.
   + intros; invnf; now apply DeclarativeTypingProperties.RedTermDeclProperties.
   + intros; invnf; change (@red_tm nf) with (@red_tm de).
     now eapply redtm_conv.
