theories/Substitution/Introductions/Reflect.v
@@ -1,0 +1,1053 @@
+From LogRel.AutoSubst Require Import core unscoped Ast Extra.
+From LogRel Require Import Utils BasicAst Computation Notations Context Closed NormalForms NormalEq Weakening UntypedReduction
+  DeclarativeTyping GenericTyping LogicalRelation Validity.
+From LogRel.LogicalRelation Require Import Escape Reflexivity Neutral Weakening Irrelevance Application Reduction Transitivity NormalRed.
+From LogRel.Substitution Require Import Irrelevance Properties SingleSubst.
+From LogRel.Substitution.Introductions Require Import Universe Var Nat SimpleArr Sigma Id Quote.
+
+Set Universe Polymorphism.
+
+Section Utils.
+
+Context `{GenericTypingProperties}.
+
+Lemma embRedTy {Γ l l' A} (h : l << l') (rA : [Γ ||-< l > A]) : [Γ ||-< l' > A].
+Proof.
+destruct rA as [pack].
+unshelve econstructor.
+- exact pack.
+- eapply Induction.LR_embedding; tea.
+Defined.
+
+Lemma embRedTyOne {Γ l A} (rA : [Γ ||-< l > A]) : [Γ ||-< one > A].
+Proof.
+destruct l; tea; now eapply (embRedTy Oi).
+Defined.
+
+Lemma dnf_closed_qNat_aux : forall Γ (rNat : [Γ ||-Nat tNat]),
+  (forall t, [Γ ||-Nat t : tNat | rNat] -> forall u, [t ⇶* u] -> dnf u -> closed0 u -> ∑ n, u = qNat n) ×
+  (forall t, NatProp rNat t -> forall u, [t ⇶* u] -> dnf u -> closed0 u -> ∑ n, u = qNat n).
+Proof.
+intros; apply NatRedInduction.
++ intros * [? Hr] Heq ? IH u Hr' Hnf Hc.
+  apply IH; tea.
+  eapply dred_red_det; tea.
+  now eapply dred_red, redtm_sound.
++ intros * Hr Hnf Hc.
+  apply dred_dnf in Hr; [subst|eauto using dnf].
+  exists 0; reflexivity.
++ intros * Hn IH u Hr Hnf Hc.
+  destruct (redalg_succ_adj _ _ Hr) as [m ->].
+  apply redalg_succ_inv in Hr.
+  inversion Hnf; subst; [|match goal with H : dne _ |- _ => inversion H end].
+  destruct (IH _ Hr) as [v Hv]; tea; subst.
+  exists (S v); reflexivity.
++ intros n [? Hne] * Hr Hnf Hc; exfalso.
+  apply convneu_whne in Hne.
+  eapply dredalg_whne in Hr; [|tea].
+  now eapply closed0_whne.
+Qed.
+
+Lemma dnf_closed_qNat : forall Γ l t u (rΓ : [|- Γ]) (rNat := natRed rΓ),
+  [Γ ||-<l> t : tNat | rNat] -> [t ⇶* u] -> dnf u -> closed0 u -> ∑ n, u = qNat n.
+Proof.
+intros * Ht Hr Hnf.
+edestruct dnf_closed_qNat_aux as [Haux ?]; eapply Haux; tea.
+Qed.
+
+Set Printing Primitive Projection Parameters.
+
+Lemma NatPropEq_diag {Γ A} {rNat : [Γ ||-Nat A]} :
+  (forall t u, [Γ ||-Nat t ≅ u : A | rNat] -> NatRedTm rNat t)
+  × (forall t u, NatPropEq rNat t u -> [Γ |- t : tNat] -> NatProp rNat t).
+Proof.
+apply NatRedEqInduction.
++ intros; econstructor; tea.
+  - now eapply lrefl.
+  - destruct redL; eauto.
++ constructor.
++ intros; now constructor.
++ intros * []; constructor.
+  constructor; tea; now eapply lrefl.
+Qed.
+
+Lemma LRTmEqRed_l : forall Γ l A t u (rA : [Γ ||-<l> A]),
+  [rA | Γ ||- t ≅ u : A] -> [rA | Γ ||- t : A].
+Proof.
+intros Γ l A t u rA.
+revert t u.
+pattern l, Γ, A, rA.
+eapply Induction.LR_rect_TyUr; clear l Γ A rA.
++ intros l Γ A rU t u [rl]; apply rl.
++ intros l Γ A rne t u [].
+  unshelve econstructor; [|tea|].
+  now eapply lrefl.
++ intros l Γ A rΠ IHdom IHcod t u []; tea.
++ intros l Γ A rNat t u [].
+  cbn; econstructor; [tea| |].
+  - now eapply lrefl.
+  - destruct redL; now eapply NatPropEq_diag.
++ intros l Γ A rEmpty t u [].
+  cbn; econstructor; [tea| |].
+  - now eapply lrefl.
+  - destruct prop; do 2 constructor.
+    * apply redL.
+    * destruct r; now eapply lrefl.
++ intros l Γ A rΣ IHdom IHcod t u []; tea.
++ intros l Γ A rId IHty IHty' t u [].
+  cbn; econstructor; [tea| |].
+  - now eapply lrefl.
+  - destruct prop; [left|right]; tea.
+    split; [apply redL|destruct r; now eapply lrefl].
+Qed.
+
+Lemma LRTmEqRed_r : forall Γ l A t u (rA : [Γ ||-<l> A]),
+  [rA | Γ ||- t ≅ u : A] -> [rA | Γ ||- u : A].
+Proof.
+intros; now eapply LRTmEqRed_l, LRTmEqSym.
+Qed.
+
+Lemma red_redtm_exp {Γ l A t t' u u'} (rA : [Γ ||-<l> A]) :
+  [Γ |- t' ⤳* t : A] -> [Γ |- u' ⤳* u : A] ->
+  [Γ ||-<l> t ≅ u : A | rA] -> [Γ ||-<l> t' ≅ u' : A | rA].
+Proof.
+intros.
+eapply transEqTerm; [|eapply transEqTerm; [|apply LRTmEqSym]].
+- apply redSubstTerm; [|tea].
+  now eapply LRTmEqRed_l.
+- tea.
+- apply redSubstTerm; [|tea].
+  now eapply LRTmEqRed_r.
+Qed.
+
+Lemma simple_betaRed {Γ l A B t a} (rΓ : [|- Γ])
+  (rA : [Γ ||-<l> A]) (rB : [Γ ||-<l> B]) :
+  [Γ,, A |- t : B⟨@wk1 Γ A⟩] ->
+  [Γ |- a : A] ->
+  [rB | Γ ||- t[a..] : B] ->
+  [rB | Γ ||- tApp (tLambda A t) a ≅ t[a..] : B].
+Proof.
+intros rt ra rta.
+apply redSubstTerm; [tea|].
+replace B with B⟨↑⟩[a..] by now bsimpl.
+eapply redtm_beta.
++ now eapply escape.
++ now rewrite wk1_ren_on in rt.
++ tea.
+Qed.
+
+Lemma simple_lambdaRed {Γ l A B t} (rΓ : [|- Γ])
+  (rA : [Γ ||-<l> A]) (rB : [Γ ||-<l> B]) (rΠ : [Γ ||-<l> arr A B])
+  (rte : forall Δ a b (ρ : Δ ≤ Γ) (rΔ : [|- Δ]) (rA := wk ρ rΔ rA) (rB := wk ρ rΔ rB),
+    [Δ ||-<l> a : A⟨ρ⟩ | rA] -> [Δ ||-<l> b : A⟨ρ⟩ | rA] -> [Δ ||-<l> a ≅ b : A⟨ρ⟩ | rA] -> [Δ ||-<l> t[a .: ρ >> tRel] ≅ t[b .: ρ >> tRel] : B⟨ρ⟩ | rB]) :
+  [Γ ||-<l> tLambda A t : arr A B | rΠ].
+Proof.
+assert (rt : forall Δ a (ρ : Δ ≤ Γ) (rΔ : [|- Δ]) (rA := wk ρ rΔ rA) (rB := wk ρ rΔ rB), [Δ ||-<l> a : A⟨ρ⟩ | rA] -> [Δ ||-<l> t[a .: ρ >> tRel] : B⟨ρ⟩ | rB]).
+{ intros; eapply LRTmEqRed_l, rte; tea.
+  now apply reflLRTmEq. }
+pose (rΠ0 := normRedΠ rΠ).
+unshelve irrelevance0; [| |apply rΠ0|reflexivity|].
+assert [Γ |- A] by now escape.
+assert [Γ |- A ≅ A].
+{ unshelve eapply escapeEq, reflLRTyEq; tea. }
+assert [|- Γ,, A] by now apply wfc_cons.
+assert [Γ,, A |- B⟨↑⟩].
+{ rewrite <- (wk1_ren_on Γ A).
+  now unshelve eapply escape, wk, rB. }
+assert [Γ,, A |- B⟨↑⟩ ≅ B⟨↑⟩].
+{ rewrite <- !(@wk1_ren_on Γ A).
+  apply convty_wk; [|unshelve eapply escapeEq, reflLRTyEq; tea].
+  now apply wfc_cons. }
+assert [Γ,, A |- t : B⟨↑⟩].
+{ replace t with t[(tRel 0) .: @wk1 Γ A >> tRel].
+  2:{ bsimpl; apply idSubst_term; intros []; reflexivity. }
+  rewrite <- (wk1_ren_on Γ A).
+  unshelve eapply escapeTerm, rt; [tea|].
+  apply var0; [now rewrite wk1_ren_on|tea]. }
+assert [Γ,, A |- t ≅ t : B⟨↑⟩].
+{ replace t with t[(tRel 0) .: @wk1 Γ A >> tRel].
+  2:{ bsimpl; apply idSubst_term; intros []; reflexivity. }
+  rewrite <- (wk1_ren_on Γ A).
+  unshelve eapply escapeEqTerm, reflLRTmEq, rt; [tea|].
+  apply var0; [now rewrite wk1_ren_on|tea]. }
+assert [Γ |- tLambda A t : arr A B].
+{ now apply ty_lam. }
+assert (forall Δ (ρ : Δ ≤ Γ), [|- Δ] -> [Δ,, A⟨ρ⟩ |- t⟨upRen_term_term ρ⟩ : B⟨ρ⟩⟨↑⟩]).
+{ intros.
+  rewrite <- (@wk_up_ren_on _ _ ρ A), <- (@wk1_ren_on Δ A⟨ρ⟩), wk_up_wk1.
+  apply ty_wk; [|now rewrite wk1_ren_on].
+  apply wfc_cons; tea; now eapply escape, wk. }
+eexists (tLambda A t).
++ apply redtmwf_refl, ty_lam; tea.
++ unshelve constructor; cbn.
+  - intros; apply reflLRTyEq.
+  - intros; irrelevance0; [|unshelve apply rt; tea].
+    bsimpl; apply rinstInst'_term.
+    irrelevance0; [reflexivity|tea].
++ cbn; apply convtm_eta; tea.
+  - constructor; tea.
+  - constructor; tea.
+  - cbn.
+    assert [Γ,, A |- tApp (tLambda A⟨↑⟩ t⟨upRen_term_term ↑⟩) (tRel 0) ⤳* t : B⟨↑⟩].
+    { replace B⟨↑⟩ with B⟨↑ >> ↑⟩[(tRel 0)..].
+      2:{ bsimpl; symmetry; now apply rinst_inst_term. }
+      set (t' := t) at 2; replace t' with t⟨upRen_term_term ↑⟩[(tRel 0)..].
+      2:{ bsimpl; apply idSubst_term; now intros []. }
+      eapply redtm_beta.
+      + rewrite <- (@wk1_ren_on Γ A); now apply wft_wk.
+      + replace B⟨↑ >> ↑⟩ with (B⟨↑⟩⟨upRen_term_term ↑⟩) by now bsimpl.
+        rewrite <- !(wk_up_wk1_ren_on Γ A A).
+        rewrite <- (wk1_ren_on Γ A).
+        apply ty_wk; [|tea]; apply wfc_cons; [tea|].
+        apply wft_wk; tea.
+      + now apply ty_var0.
+    }
+    eapply convtm_exp; tea.
++ cbn; intros.
+  assert (Hrw : B⟨ρ⟩ = B⟨↑⟩[a .: ρ >> tRel]).
+  { bsimpl; apply rinstInst'_term. }
+  eapply (redSubstTerm (u := t[a .: ρ >> tRel])); tea.
+  - irrelevance0; [|unshelve apply rt; tea].
+    bsimpl; apply rinstInst'_term.
+    irrelevance0; [reflexivity|tea].
+  - replace t[a .: ρ >> tRel] with t⟨upRen_term_term ρ⟩[a..] by now bsimpl.
+    rewrite <- Hrw.
+    replace B⟨ρ⟩ with B⟨ρ⟩⟨↑⟩[a..].
+    2:{ bsimpl; symmetry; apply rinstInst'_term. }
+    apply redtm_beta; [now eapply escape, wk| |now eapply escapeTerm].
+    now eauto.
++ cbn; intros.
+  assert (Hrw : B⟨ρ⟩ = B⟨↑⟩[a .: ρ >> tRel]).
+  { bsimpl; apply rinstInst'_term. }
+  unshelve (irrelevance0; [tea|]); [shelve|now apply wk|].
+  unshelve eapply (LREqTermHelper (G' := B⟨ρ⟩)). 1-2: shelve.
+  - now apply wk.
+  - unshelve eapply simple_betaRed; first [now apply wk|now eapply escapeTerm|tea].
+    * rewrite wk1_ren_on; now eauto.
+    * replace (t⟨upRen_term_term ρ⟩[a..]) with t[a .: ρ >> tRel] by now bsimpl.
+      apply rt.
+      irrelevance0; [reflexivity|apply ha].
+  - unshelve eapply simple_betaRed; first [now apply wk|now eapply escapeTerm|tea].
+    * rewrite wk1_ren_on; now eauto.
+    * replace (t⟨upRen_term_term ρ⟩[b..]) with t[b .: ρ >> tRel] by now bsimpl.
+      apply rt.
+      irrelevance0; [reflexivity|apply hb].
+  - apply reflLRTyEq.
+  - replace (t⟨upRen_term_term ρ⟩[a..]) with t[a .: ρ >> tRel] by now bsimpl.
+    replace (t⟨upRen_term_term ρ⟩[b..]) with t[b .: ρ >> tRel] by now bsimpl.
+    apply rte; (irrelevance0; [reflexivity|]).
+    { apply ha. }
+    { apply hb. }
+    { apply eq. }
+Qed.
+
+Lemma tAndRed {Γ l A B} (rΓ : [|- Γ])
+  (rA : [Γ ||-<l> A]) (rB : [Γ ||-<l> B]) : [Γ ||-<l> tAnd A B].
+Proof.
+assert [Γ |- A] by now eapply escape.
+assert [|- Γ,, A] by gen_typing.
+assert [Γ |- B] by now eapply escape.
+assert [Γ,, A |- B⟨↑⟩].
+{ rewrite <- (@wk1_ren_on Γ A); apply wft_wk; tea. }
+eapply LRSig'; econstructor.
++ now apply redtywf_refl, wft_sig.
++ unshelve eapply escapeEq, reflLRTyEq; tea.
++ apply convty_sig; tea.
+  - unshelve eapply escapeEq, reflLRTyEq; tea.
+  - rewrite <- (@wk1_ren_on Γ A); apply convty_wk; tea.
+    unshelve eapply escapeEq, reflLRTyEq; tea.
++ unshelve econstructor; tea.
+  - intros; now eapply wk.
+  - intros ? a **.
+    assert (Hrw : B⟨ρ⟩ = B⟨↑⟩[a .: ρ >> tRel]).
+    { bsimpl; apply rinstInst'_term. }
+    rewrite <- Hrw; now eapply wk.
+  - intros.
+    assert (Hrw : forall a, B⟨ρ⟩ = B⟨↑⟩[a .: ρ >> tRel]).
+    { intros; bsimpl; apply rinstInst'_term. }
+    irrelevance0; [apply Hrw|].
+    rewrite <- Hrw; unshelve apply wkEq, reflLRTyEq; tea.
+Qed.
+
+Lemma tAndRedEq {Γ l A A' B B'} (rΓ : [|- Γ]) (rΣ : [Γ ||-<l> tAnd A B])
+  (rA : [Γ ||-<l> A]) (tA' : [Γ |- A']) (rB : [Γ ||-<l> B]) (tB' : [Γ |- B']) (rAA' : [rA | Γ ||- A ≅ A']) (rBB' : [rB | Γ ||- B ≅ B'])
+  : [rΣ | Γ ||- tAnd A B ≅ tAnd A' B'].
+Proof.
+pose (rΣ0 := normRedΣ rΣ).
+unshelve (irrelevance0; [reflexivity|]); [|apply rΣ0|].
+unshelve econstructor; [shelve|shelve|..].
++ apply redtywf_refl,  wft_sig; tea.
+  rewrite <- !(@wk1_ren_on Γ A').
+  apply wft_wk; tea.
+  now eapply wfc_cons.
++ cbn; now eapply escapeEq.
++ cbn; eapply convty_sig.
+  - now eapply escape.
+  - now eapply escapeEq.
+  - rewrite <- !(@wk1_ren_on Γ A).
+    apply convty_wk; [|now eapply escapeEq].
+    apply wfc_cons; tea; now eapply escape.
++ cbn; split.
+  - intros.
+    irrelevance0; [reflexivity|]; now unshelve eapply wkEq.
+  - intros.
+    assert (Hrw : forall B, B⟨ρ⟩ = B⟨↑⟩[a .: ρ >> tRel]).
+    { intros; bsimpl; apply rinstInst'_term. }
+    irrelevance0; [apply Hrw|].
+    rewrite <- Hrw.
+    now unshelve eapply wkEq.
+Qed.
+
+Lemma tAndURed {Γ l A B} (rΓ : [|- Γ])
+  (rU : [Γ ||-<l> U]) (rA : [Γ ||-<l> A : U | rU]) (rB : [Γ ||-<l> B : U | rU]) :
+  [Γ ||-<l> tAnd A B : U | rU].
+Proof.
+unshelve (irrelevance0; [reflexivity|]); [|apply (LRU_ (redUOne rΓ))|].
+assert [Γ |- A : U] by now eapply escapeTerm.
+assert [|- Γ,, A] by gen_typing.
+assert [Γ |- B : U] by now eapply escapeTerm.
+econstructor.
++ apply redtmwf_refl, ty_sig.
+  - now unshelve eapply escapeTerm.
+  - rewrite <- (@wk1_ren_on Γ A).
+    change U with U⟨@wk1 Γ A⟩; eapply ty_wk; tea.
++ constructor.
++ apply convtm_sig; tea.
+  - now eapply escapeEqTerm, reflLRTmEq.
+  - rewrite <- (@wk1_ren_on Γ A).
+    change U with U⟨@wk1 Γ A⟩; eapply convtm_wk; tea.
+    now eapply escapeEqTerm, reflLRTmEq.
++ cbn.
+  unshelve refine (LRCumulative (tAndRed _ _ _)); tea.
+  - assert (rA' : [ LRU_ (redUOne rΓ) | Γ ||- A : U]) by now irrelevance0.
+    destruct rA' as [? ? ? ? r]; apply r.
+  - assert (rB' : [ LRU_ (redUOne rΓ) | Γ ||- B : U]) by now irrelevance0.
+    destruct rB' as [? ? ? ? r]; apply r.
+Qed.
+
+Lemma tAndURedEq {Γ l A A' B B'} (rΓ : [|- Γ])
+  (rU : [Γ ||-<l> U])
+  (rAA' : [Γ ||-<l> A ≅ A' : U | rU]) (rBB' : [Γ ||-<l> B ≅ B' : U | rU]) : [Γ ||-<l> tAnd A B ≅ tAnd A' B' : U | rU].
+Proof.
+intros.
+pose (rU' := LRU_ (redUOne rΓ)).
+unshelve (irrelevance0; [reflexivity|]); [|apply rU'|].
+unshelve eapply LRTmEqIrrelevant' in rAA'; [..|reflexivity]; [|apply rU'|].
+unshelve eapply LRTmEqIrrelevant' in rBB'; [..|reflexivity]; [|apply rU'|].
+assert (rA : [Γ ||-<one> A : U | rU']) by apply rAA'.
+assert (rA' : [Γ ||-<one> A' : U | rU']) by apply rAA'.
+assert (rB : [Γ ||-<one> B : U | rU']) by apply rBB'.
+assert (rB' : [Γ ||-<one> B' : U | rU']) by apply rBB'.
+unshelve econstructor.
++ refine (tAndURed rΓ rU' rA rB).
++ refine (tAndURed rΓ rU' rA' rB').
++ unshelve refine (tAndRed _ _ _); tea.
+  - destruct rA as [? ? ? ? r]; apply r.
+  - destruct rB as [? ? ? ? r]; apply r.
++ assert (Hrw : forall rec t A (R : [Γ ||-U< one > A]) (p : [rec | Γ ||-U t : A | R]), whnf t -> URedTm.te p = t).
+  { intros; symmetry; eapply red_whnf; [|tea].
+    now eapply redtm_sound, tmr_wf_red, URedTm.red. }
+  rewrite !Hrw; try now constructor.
+  apply convtm_and; first [now eapply escapeTerm|now eapply escapeEqTerm].
++ refine (tAndRed _ _ _); tea.
+  - destruct rA' as [? ? ? ? r]; apply r.
+  - destruct rB' as [? ? ? ? r]; apply r.
++ cbn.
+  unshelve eapply tAndRedEq; tea.
+  - apply rA.
+  - apply rB.
+  - now eapply wft_term, escapeTerm.
+  - now eapply wft_term, escapeTerm.
+  - destruct rAA'.
+    destruct rA; cbn.
+    unshelve (irrelevance0; [reflexivity|]).
+    * shelve.
+    * refine (embRedTyOne relL).
+    * apply relEq.
+  - destruct rBB'.
+    destruct rB; cbn.
+    unshelve (irrelevance0; [reflexivity|]).
+    * shelve.
+    * refine (embRedTyOne relL).
+    * apply relEq.
+Qed.
+
+Lemma tIsNilRed {Γ l t} (rΓ : [|- Γ])
+  (rNat := natRed rΓ)
+  (rU : [Γ ||-<one> U])
+  (rt : [Γ ||-<l> t : tNat | rNat]) :
+  [rU | Γ ||- tIsNil t : U].
+Proof.
+unshelve eapply Id.IdRedU.
++ now apply natRed.
++ irrelevance0; [reflexivity|]; now unshelve apply natTermRed.
++ tea.
++ unshelve eapply zeroRed; tea.
+Qed.
+
+Lemma tIsNilRedEq {Γ l t t'} (rΓ : [|- Γ])
+  (rNat := natRed rΓ)
+  (rU : [Γ ||-<one> U])
+  (rt : [Γ ||-<l> t ≅ t' : tNat | rNat]) :
+  [rU | Γ ||- tIsNil t ≅ tIsNil t' : U].
+Proof.
+unshelve eapply Id.IdCongRedU.
++ now apply natRed.
++ now apply natRed.
++ irrelevance0; [reflexivity|]; now unshelve apply natTermRed.
++ irrelevance0; [reflexivity|]; now unshelve apply natTermRed.
++ eapply reflLRTmEq; irrelevance0; [reflexivity|]; now unshelve apply natTermRed.
++ eapply LRTmEqRed_l, rt.
++ eapply LRTmEqRed_r, rt.
++ eapply rt.
++ now eapply zeroRed.
++ now eapply zeroRed.
++ now eapply zeroRedEq.
+Qed.
+
+Lemma tIsValRed {Γ l t v} (rΓ : [|- Γ])
+  (rNat := natRed rΓ)
+  (rU : [Γ ||-<one> U])
+  (rt : [Γ ||-<l> t : tNat | rNat])
+  (rv : [Γ ||-<l> v : tNat | rNat]) :
+  [rU | Γ ||- tIsVal t v : U].
+Proof.
+unshelve eapply Id.IdRedU.
++ now apply natRed.
++ irrelevance0; [reflexivity|]; now unshelve apply natTermRed.
++ tea.
++ unshelve eapply succRed, rv.
+Qed.
+
+Lemma tIsValRedEq {Γ l t t' v v'} (rΓ : [|- Γ])
+  (rNat := natRed rΓ)
+  (rU : [Γ ||-<one> U])
+  (rt : [Γ ||-<l> t ≅ t' : tNat | rNat])
+  (rv : [Γ ||-<l> v ≅ v' : tNat | rNat]) :
+  [rU | Γ ||- tIsVal t v ≅ tIsVal t' v' : U].
+Proof.
+pose (rU' := LRU_ (redUOne rΓ)).
+unshelve (irrelevance0; [reflexivity|]); [|exact rU'|].
+clear rU; rename rU' into rU.
+assert [rU | Γ ||- tNat : U].
+{ irrelevance0; [reflexivity|].
+  now unshelve apply natTermRed. }
+assert [rU | Γ ||- tNat ≅ tNat : U] by now apply reflLRTmEq.
+assert (rS : [rNat | Γ ||- tSucc v ≅ tSucc v' : tNat]).
+{ apply succRedEq.
+  - eapply LRTmEqRed_l, rv.
+  - eapply LRTmEqRed_r, rv.
+  - eapply rv. }
+unshelve eapply Id.IdCongRedU; tea.
++ now apply natRed.
++ now apply natRed.
++ eapply LRTmEqRed_l, rt.
++ eapply LRTmEqRed_r, rt.
++ apply rt.
++ eapply LRTmEqRed_l, rS.
++ eapply LRTmEqRed_r, rS.
++ eapply rS.
+Qed.
+
+Lemma tShiftRed {Γ l t} (rPNat : [Γ ||-<l> tPNat])
+  (rt : [rPNat | Γ ||- t : tPNat]) : [rPNat | Γ ||- tShift t : tPNat].
+Proof.
+assert (rΓ : [|- Γ]).
+{ eapply wfc_wft; now eapply escape. }
+pose (rNat := natRed (l := l) rΓ).
+unshelve eapply simple_lambdaRed; tea; intros.
+cbn - [rB]; unshelve eapply (SimpleArr.simple_appcongTerm (F := tNat)).
++ tea.
++ change (arr tNat tNat⟨ρ⟩) with (arr tNat tNat)⟨ρ⟩.
+  now eapply (wk ρ).
++ assert (Hrw : forall a, t⟨ρ⟩ = t⟨↑⟩[a .: ρ >> tRel]).
+  { intros; bsimpl; apply rinstInst'_term. }
+  rewrite <- !Hrw.
+  now apply reflLRTmEq, wkTerm.
++ eapply succRed; tea.
++ eapply succRed; tea.
++ eapply succRedEq; tea.
+Qed.
+
+Lemma redtm_shift_app {Γ t u} :
+  [Γ |- t : arr tNat tNat] ->
+  [Γ |- u : tNat] ->
+  [Γ |- tApp (tShift t) u ⤳* tApp t (tSucc u) : tNat].
+Proof.
+intros; unfold tShift.
+assert [|- Γ] by gen_typing.
+assert [|- Γ,, tNat] by gen_typing.
+assert [Γ,, tNat |- tNat] by now apply wft_nat.
+replace (tApp t (tSucc u)) with (tApp t⟨↑⟩ (tSucc (tRel 0)))[u..] by now bsimpl.
+change tNat with tNat[u..].
+eapply redtm_beta.
++ now apply wft_nat.
++ cbn; apply (ty_simple_app (A := tNat)); tea.
+  - rewrite <- (@wk1_ren_on Γ tNat t).
+    change (arr tNat tNat) with (arr tNat tNat)⟨@wk1 Γ tNat⟩.
+    now apply ty_wk.
+  - apply ty_succ, ty_var; tea.
+    change tNat with tNat⟨↑⟩ at 2; constructor.
++ tea.
+Qed.
+
+Lemma tShift_ren : forall t ρ, (tShift t)⟨ρ⟩ = tShift (t⟨ρ⟩).
+Proof.
+intros; unfold tShift; cbn; do 2 f_equal.
+now bsimpl.
+Qed.
+
+Lemma tShiftRedEq {Γ l t t'} (rPNat : [Γ ||-<l> tPNat])
+  (rt : [rPNat | Γ ||- t ≅ t' : tPNat]) : [rPNat | Γ ||- tShift t ≅ tShift t' : tPNat].
+Proof.
+assert (rΓ : [|- Γ]).
+{ eapply wfc_wft; now eapply escape. }
+pose (rPNat0 := normRedΠ rPNat).
+unshelve irrelevance0; [| |apply rPNat0|reflexivity|].
+unshelve (eapply LRTmEqIrrelevant' in rt; [|reflexivity]); [|exact rPNat0|].
+assert (Hrw : forall t R (p : [Γ ||-Π t : tPNat | R]), whnf t -> PiRedTm.nf p = t).
+{ intros; symmetry; eapply red_whnf; tea.
+    now eapply redtm_sound, tmr_wf_red, PiRedTm.red. }
+unshelve econstructor.
++ eapply (tShiftRed rPNat0).
+  irrelevance0; [reflexivity|]; now eapply LRTmEqRed_l.
++ eapply (tShiftRed rPNat0).
+  irrelevance0; [reflexivity|]; now eapply LRTmEqRed_r.
++ rewrite !Hrw; cbn; try now constructor.
+  assert [Γ |- tNat] by now apply wft_nat.
+  assert [Γ |- tNat ≅ tNat] by now apply convty_term, convtm_nat.
+  apply convtm_lam; tea.
+  assert (rΓNat : [|- Γ,, tNat]) by gen_typing.
+  assert [natRed (l := l) rΓNat | _ ||- tRel 0 : tNat].
+  { apply var0; [reflexivity|]; gen_typing. }
+  assert [natRed (l := l) rΓNat | _ ||- tSucc (tRel 0) : tNat].
+  { now apply succRed. }
+  assert [natRed (l := l) rΓNat | _ ||- tSucc (tRel 0) ≅ tSucc (tRel 0) : tNat].
+  { apply succRedEq; tea; now apply reflLRTmEq. }
+  rewrite <- (@wk1_ren_on Γ tNat t), <- (@wk1_ren_on Γ tNat t').
+  unshelve eapply escapeEqTerm, (SimpleArr.simple_appcongTerm (F := tNat)); tea.
+  - now apply natRed.
+  - change (arr tNat tNat) with (arr tNat tNat)⟨@wk1 Γ tNat⟩.
+    now apply wk.
+  - apply wkTermEq, rt.
++ intros.
+  rewrite !Hrw; try now constructor; cbn.
+  unfold ren1, Ren1_well_wk.
+  rewrite !(tShift_ren).
+  eapply red_redtm_exp.
+  - apply redtm_shift_app; [|now eapply escapeTerm].
+    change (arr tNat tNat) with (arr tNat tNat)⟨ρ⟩.
+    apply ty_wk; [tea|].
+    now eapply escapeTerm, LRTmEqRed_l.
+  - apply redtm_shift_app; [|now eapply escapeTerm].
+    change (arr tNat tNat) with (arr tNat tNat)⟨ρ⟩.
+    apply ty_wk; [tea|].
+    now eapply escapeTerm, LRTmEqRed_r.
+  - assert [natRed (l := l) h | Δ ||- a : tNat].
+    { irrelevance0; [reflexivity|]; apply ha. }
+    assert [natRed (l := l) h | Δ ||- tSucc a : tNat].
+    { now apply succRed. }
+    assert [natRed (l := l) h | Δ ||- tSucc a ≅ tSucc a : tNat].
+    { apply succRedEq; tea; now apply reflLRTmEq. }
+    unshelve eapply (SimpleArr.simple_appcongTerm (F := tNat)); tea.
+    * cbn; change (tProd tNat tNat) with (tProd tNat tNat)⟨ρ⟩.
+      apply wk; tea.
+    * apply wkTermEq, rt.
+Qed.
+
+Lemma tEvalZeroRedEq {Γ l t v} (rΓ : [|- Γ])
+  (rNat := natRed rΓ) (rNatNat := SimpleArr.ArrRedTy rNat rNat)
+  (rU : [Γ ||-<one> U])
+  (rt : [Γ ||-<l> t : tPNat | rNatNat])
+  (rv : [Γ ||-<l> v : tNat | rNat]) :
+  [Γ ||-<one> tEval t tZero v ≅ tIsVal (tApp t tZero) v : U | rU].
+Proof.
+intros; apply redSubstTerm.
++ unshelve eapply tIsValRed; [..|tea].
+  unshelve eapply SimpleArr.simple_appTerm.
+  - shelve.
+  - now unshelve apply natRed.
+  - apply SimpleArr.ArrRedTy; now apply natRed.
+  - irrelevance0; [reflexivity|]; apply rt.
+  - unshelve irrelevance0; [..|reflexivity|]; [|tea|]; unshelve eapply zeroRed; tea.
++ apply redtm_evalBranchZero.
+  - unshelve eapply escapeTerm, rt.
+  - unshelve eapply escapeTerm, rv.
+Qed.
+
+Lemma tEvalSuccRedEq {Γ l t k v} (rΓ : [|- Γ])
+  (rNat := natRed rΓ) (rNatNat := SimpleArr.ArrRedTy rNat rNat)
+  (rU : [Γ ||-<one> U])
+  (rt : [Γ ||-<l> t : tPNat | rNatNat])
+  (rk : [Γ ||-<l> k : tNat | rNat])
+  (rv : [Γ ||-<l> v : tNat | rNat])
+  (rrec : [rU | Γ ||- tEval (tShift t) k v : U]) :
+  [Γ ||-<one> tEval t (tSucc k) v ≅ tAnd (tIsNil (tApp t k)) (tEval (tShift t) k v) : U | rU].
+Proof.
+apply redSubstTerm.
++ apply tAndURed; tea.
+  unshelve eapply tIsNilRed; [shelve|tea|].
+  eapply SimpleArr.simple_appTerm; tea.
++ apply redtm_evalBranchSucc.
+  - now eapply escapeTerm.
+  - now eapply escapeTerm.
+  - now eapply escapeTerm.
+Qed.
+
+Lemma tEvalNeuRedEq {Γ t t' k k' v v'} (rΓ : [|- Γ])
+  (rU : [Γ ||-<one> U])
+  (rt : [Γ |- t : tPNat])
+  (rt' : [Γ |- t' : tPNat])
+  (rtt' : [Γ |- t ≅ t' : tPNat])
+  (rk : [Γ |- k : tNat])
+  (rk' : [Γ |- k' : tNat])
+  (rkk' : [Γ |- k ~ k' : tNat])
+  (rv : [Γ |- v : tNat])
+  (rv' : [Γ |- v' : tNat])
+  (rvv' : [Γ |- v ≅ v' : tNat]) :
+  [Γ ||-<one> tEval t k v ≅ tEval t' k' v' : U | rU].
+Proof.
+apply neuTermEq.
++ apply ty_eval; tea.
++ apply ty_eval; tea.
++ apply tEval_cong; tea.
+Qed.
+
+Lemma tEvalRedEq {Γ l t t' k k' v v'} (rΓ : [|- Γ])
+  (rNat : [Γ ||-<l> tNat]) (rPNat : [Γ ||-<l> tPNat])
+  (rU : [Γ ||-<one> U])
+  (rt : [Γ ||-<l> t ≅ t' : tPNat | rPNat])
+  (rk : [Γ ||-<l> k ≅ k' : tNat | rNat])
+  (rv : [Γ ||-<l> v ≅ v' : tNat | rNat]) :
+  [Γ ||-<one> tEval t k v ≅ tEval t' k' v' : U | rU].
+Proof.
+assert (Rnat : [Γ ||-Nat tNat]).
+{ unshelve constructor; now apply redtywf_refl, wft_nat. }
+pose (rNat' := LRNat_ l Rnat).
+unshelve eapply LRTmEqIrrelevant' in rk; [..|exact rNat'| |reflexivity].
+unshelve eapply LRTmEqIrrelevant' in rv; [..|exact rNat'| |reflexivity].
+clear rNat; rename rNat' into rNat.
+assert [rNat | Γ ||- v : tNat] by now eapply LRTmEqRed_l.
+assert [rNat | Γ ||- v' : tNat] by now eapply LRTmEqRed_r.
+revert t t' rt.
+assert (Hk : [Γ |- k : tNat]) by now eapply escapeTerm, LRTmEqRed_l.
+assert (Hk' : [Γ |- k' : tNat]) by now eapply escapeTerm, LRTmEqRed_r.
+revert Hk Hk'.
+pattern k, k'.
+match goal with |- ?F _ _ => pose (P := F) end.
+revert k k' rk.
+cut ((forall k k', NatRedTmEq Rnat k k' -> P k k') × (forall k k', NatPropEq Rnat k k' -> P k k')).
+{ intros [IH]; apply IH. }
+apply NatRedEqInduction; unfold P.
++ intros k k' * [] [] ?? IH ?? t t' rt.
+  eapply red_redtm_exp; [| |now apply IH]; apply redtm_evalArg; tea.
+  - now eapply escapeTerm, LRTmEqRed_l.
+  - now eapply escapeTerm.
+  - now eapply escapeTerm, LRTmEqRed_r.
+  - now eapply escapeTerm.
++ intros ?? t t' rt.
+  assert [rPNat | Γ ||- t : tPNat] by now eapply LRTmEqRed_l.
+  assert [rPNat | Γ ||- t' : tPNat] by now eapply LRTmEqRed_r.
+  eapply red_redtm_exp.
+  - eapply redtm_evalBranchZero; now unshelve eapply escapeTerm.
+  - eapply redtm_evalBranchZero; now unshelve eapply escapeTerm.
+  - unshelve eapply tIsValRedEq; [tea|tea| |now (irrelevance0; [reflexivity|tea])].
+    eapply SimpleArr.simple_appcongTerm; tea.
+    * now unshelve eapply zeroRed.
+    * now eapply zeroRed.
+    * now eapply zeroRedEq.
++ intros k k' rk IH ?? t t' rt.
+  assert [rPNat | Γ ||- t : tPNat] by now eapply LRTmEqRed_l.
+  assert [rPNat | Γ ||- t' : tPNat] by now eapply LRTmEqRed_r.
+  assert [Γ |- k : tNat].
+  { destruct rk; now eapply redtm_ty_src, tmr_wf_red. }
+  assert [Γ |- k' : tNat].
+  { destruct rk; now eapply redtm_ty_src, tmr_wf_red. }
+  eapply red_redtm_exp.
+  - eapply redtm_evalBranchSucc; try now unshelve eapply escapeTerm.
+    tea.
+  - eapply redtm_evalBranchSucc; try now unshelve eapply escapeTerm.
+    tea.
+  - apply tAndURedEq; tea.
+    * unshelve eapply tIsNilRedEq; [shelve|tea|].
+      assert [rNat | Γ ||- k ≅ k' : tNat] by apply rk.
+      unshelve eapply (SimpleArr.simple_appcongTerm (F := tNat)); tea.
+      { now eapply LRTmEqRed_l. }
+      { now eapply LRTmEqRed_r. }
+    * apply IH; tea.
+      now apply tShiftRedEq.
++ intros k k' rk ?? t t' rt.
+  assert [rPNat | Γ ||- t : tPNat] by now eapply LRTmEqRed_l.
+  assert [rPNat | Γ ||- t' : tPNat] by now eapply LRTmEqRed_r.
+  apply tEvalNeuRedEq; first [assumption|now eapply escapeTerm|now eapply escapeEqTerm|idtac].
+  apply rk.
+Qed.
+
+(*
+Lemma tEvalZeroBranchRed {Γ v} (rΓ : [|- Γ])
+  (rNat : [Γ ||-<one> tNat]) (rP : [Γ ||-<one> arr tPNat U])
+  (rv : [rNat | Γ ||- v : tNat]) :
+  [rP | Γ ||- tLambda tPNat (tIsVal (tApp (tRel 0) tZero) v⟨↑⟩) : arr tPNat U].
+Proof.
+unshelve eapply simple_lambdaRed; tea.
++ apply SimpleArr.ArrRedTy; now apply natRed.
++ now apply LRU_, redUOne.
++ intros.
+  rewrite !tIsVal_subst; cbn - [rB].
+  assert (Hrw : forall a, v⟨↑⟩[a .: ρ >> tRel] = v⟨ρ⟩).
+  { intros x; bsimpl; symmetry; apply rinstInst'_term. }
+  rewrite !Hrw.
+Admitted.
+
+Lemma tEvalSuccBranchRed {Γ} (rΓ : [|- Γ]) (rS : [Γ ||-<one> arr tNat (arr (arr tPNat U) (arr tPNat U))]) :
+  [rS | Γ ||- tLambda tNat (tLambda (arr tPNat U) (tLambda tPNat
+    (tAnd (tIsNil (tApp (tRel 0) (tRel 2))) (tApp (tRel 1) (tShift (tRel 0)))))) : arr tNat (arr (arr tPNat U) (arr tPNat U))].
+Proof.
+unshelve eapply simple_lambdaRed; tea.
++ now apply natRed.
++ do 2 apply SimpleArr.ArrRedTy; admit.
++ intros.
+  cbn - [tAnd tIsNil].
+  rewrite !tAnd_subst, !tIsNil_subst.
+  cbn - [tAnd tIsNil].
+  admit.
+Admitted.
+*)
+
+Lemma tEvalRed {Γ l t k v} (rΓ : [|- Γ])
+  (rNat := natRed rΓ) (rNatNat := SimpleArr.ArrRedTy rNat rNat)
+  (rU : [Γ ||-<one> U])
+  (rt : [Γ ||-<l> t : tPNat | rNatNat])
+  (rk : [Γ ||-<l> k : tNat | rNat])
+  (rv : [Γ ||-<l> v : tNat | rNat]) :
+  [Γ ||-<one> tEval t k v : U | rU].
+Proof.
+eapply LRTmEqRed_l, tEvalRedEq.
++ tea.
++ now eapply reflLRTmEq.
++ now eapply reflLRTmEq.
++ now eapply reflLRTmEq.
+Qed.
+
+Definition evalValid {Γ l t k r} (vΓ : [||-v Γ])
+  (vNat := natValid (l := l) vΓ)
+  (vArr := simpleArrValid vΓ vNat vNat)
+  (vt : [Γ ||-v< l > t : tPNat | vΓ | vArr ])
+  (vk : [Γ ||-v< l > k : tNat | vΓ | vNat ])
+  (vr : [Γ ||-v< l > r : tNat | vΓ | vNat ]) :
+  [Γ ||-v< one > tEval t k r | vΓ].
+Proof.
+assert (vEval : forall Δ σ (vΔ : [|- Δ]) (vσ : [vΓ | Δ ||-v σ : Γ | vΔ]),
+  [Δ ||-< one > tEval t[σ] k[σ] r[σ]]).
+{ intros Δ σ vΔ **.
+  unshelve epose (rU := LRU_ (redUOne _)); [|tea|].
+  enough (rEval : [rU | Δ ||- tEval t[σ] k[σ] r[σ] : U]).
+  { destruct rEval; apply (embRedTyOne rel). }
+  unshelve eapply tEvalRed; tea.
+  - destruct vt as [vt _].
+    irrelevance0; [reflexivity|]; now unshelve apply vt.
+  - destruct vk as [vk _].
+    irrelevance0; [reflexivity|]; now unshelve apply vk.
+  - destruct vr as [vr _].
+    irrelevance0; [reflexivity|]; now unshelve apply vr.
+}
+unshelve econstructor.
++ intros Δ σ vΔ **.
+  rewrite tEval_subst.
+  now unshelve eapply vEval.
++ intros Δ σ σ' **.
+  unshelve epose (rU := LRU_ (redUOne _)); [|tea|].
+  unshelve (irrelevance0; [symmetry; apply tEval_subst|]); [|now eapply vEval|].
+  rewrite tEval_subst with (σ := σ').
+  enough (rEval : [rU | Δ ||- tEval t[σ] k[σ] r[σ] ≅ tEval t[σ'] k[σ'] r[σ'] : U]).
+  { destruct rEval.
+    unshelve (irrelevance0; [reflexivity|]).
+    * shelve.
+    * refine (embRedTyOne relL).
+    * apply relEq. }
+  unshelve eapply tEvalRedEq.
+  - shelve.
+  - now unshelve apply natRed.
+  - now unshelve (apply SimpleArr.ArrRedTy; apply natRed).
+  - tea.
+  - destruct vt as [_ vt].
+    irrelevance0; [reflexivity|]; now apply vt.
+  - destruct vk as [_ vk].
+    irrelevance0; [reflexivity|]; now apply vk.
+  - destruct vr as [_ vr].
+    irrelevance0; [reflexivity|]; now apply vr.
+  Unshelve. all: tea.
+Qed.
+
+End Utils.
+
+Section ReflectValid.
+
+Context `{GenericTypingProperties}.
+Context {SN : SNTypingProperties ta _ _ _ _ _}.
+
+(*
+Lemma ReflectRed : forall Γ l t u (rΓ : [|- Γ])
+  (rNat := natRed rΓ) (rNatNat := SimpleArr.ArrRedTy rNat rNat)
+  (rTotal : [Γ ||-<l> tTotal t u]),
+  [Γ ||-<l> t : arr tNat tNat | rNatNat] ->
+  [Γ ||-<l> u : tNat | rNat] ->
+  [Γ ||-<l> run model : arr tNat (arr tNat tPNat) | SimpleArr.ArrRedTy rNat (SimpleArr.ArrRedTy rNat rNatNat)] ->
+  [Γ ||-<l> tReflect t u : tTotal t u | rTotal].
+Proof.
+intros * rt ru rrun.
+pose (rTotal' := normRedΣ0 (Induction.invLRΣ rTotal)); refold.
+fold (tTotal t u) in rTotal'.
+eapply LRTmRedIrrelevant' with (lrA := LRSig' rTotal'); [reflexivity|].
+destruct (nf_eval rt) as [r [Hrnf [Hr Hrconv]]].
+destruct (nf_eval ru) as [n [Hnnf [Hn Hnconv]]].
+remember (is_closedn 0 r) as cr eqn:Hcr; symmetry in Hcr.
+remember (is_closedn 0 n) as cn eqn:Hcn; symmetry in Hcn.
+remember (andb cr cn) as cb eqn:Hcb; symmetry in Hcb; destruct cb.
++ destruct cr; [|cbn in Hcb; congruence].
+  destruct cn; [|cbn in Hcb; congruence].
+  assert (∑ n₀, n = qNat n₀) as [n₀]; [|subst].
+  { eapply dnf_closed_qNat; [apply ru| | |]; tea. }
+  clear Hcb Hn Hcn.
+  assert (rapp : [rNat | _ ||- tApp t u : tNat]).
+  { eapply SimpleArr.simple_appTerm; tea. }
+  assert (Heval : ∑ m k, eval true (tApp (erase t) u) k = Some (qNat m)).
+  { admit. }
+  destruct Heval as (m&k&Heval).
+(*   eapply (redSubstTerm (u := qTotal (model.(quote) (erase r)) n₀ k m)). *)
+(*
+  eapply LRTmRedConv.
+(*   - cbn; unfold qTotal. *)
+(*   unshelve eexists (qTotal (model.(quote) (erase r)) n₀ k m) _. *)
+admit.
+  - intros; unshelve irrelevance0; [exact l| |now apply natRed|reflexivity|].
+    eexists (qNat k); [|now apply convtm_qNat|now apply qNatRed].
+    split; [now apply ty_qNat|].
+    unfold ren1, Ren1_well_wk; rewrite qTotal_ren.
+    apply redtm_fst_beta.
+    * gen_typing.
+    * admit.
+    * now apply ty_qNat.
+    * rewrite tEval_subst; cbn; rewrite run_subst, quote_subst, !qNat_subst, erase_is_closed0_subst_id; tea.
+      admit.
+  - admit.
+  - admit.
+  - admit.
+  - admit.
+*)
+admit.
++ assert ([Γ |-[ ta ] run model : arr tNat (arr tNat tPNat)]).
+  { unshelve eapply escapeTerm; tea. }
+(*
+  assert [Γ |- tTotal r n ≅ tTotal t u].
+  { eapply convty_term, tTotal_cong.
+    + admit.
+    + admit.
+  }
+*)
+  eapply redSubstTerm; [|eapply redtm_reflect; tea]; try now eapply escapeTerm.
+  apply neuTerm.
+  - eapply ty_conv; [eapply ty_reflect; first [now eapply urefl|tea]|tea].
+    eapply convty_term, tTotal_cong.
+    admit.
+    admit.
+  - assert ((~ is_true (is_closedn 0 r)) + (~ is_true (is_closedn 0 n))).
+    { destruct (is_closedn 0 r); [|left; congruence].
+      destruct (is_closedn 0 n); [|right; congruence].
+      subst; cbn in Hcb; congruence. }
+    eapply convneu_reflect; first [now eapply urefl|now symmetry|tea].
+Admitted.
+*)
+
+Lemma neuTermEqRed {Γ l A t t' n n'} (RA : [Γ ||-<l> A]) :
+  [Γ |- t ⤳* n : A] ->
+  [Γ |- t' ⤳* n' : A] ->
+  [Γ |- n : A] -> [Γ |- n' : A] -> [Γ |- n ~ n' : A] -> [Γ ||-<l> t ≅ t' : A | RA].
+Proof.
+intros Ht Ht' Hn Hn' Hnn'.
+eapply transEqTerm; [|eapply LRTmEqSym, transEqTerm]; [| |eapply LRTmEqSym, neuTermEq]; [..|tea]; tea.
+- eapply redSubstTerm; [|tea]; try now eapply escapeTerm.
+  eapply neuTerm; [tea|now eapply lrefl].
+- eapply redSubstTerm; [|tea]; try now eapply escapeTerm.
+  eapply neuTerm; [tea|now eapply urefl].
+Qed.
+
+Lemma ReflectRedEq : forall Γ l t t' u u' (rΓ : [|- Γ]) (rNat := natRed rΓ) (rNatNat := SimpleArr.ArrRedTy rNat rNat)
+  (rTotal : [Γ ||-<l> tTotal t u]),
+  [Γ ||-<l> t : arr tNat tNat | rNatNat ] ->
+  [Γ ||-<l> t' : arr tNat tNat | rNatNat ] ->
+  [Γ ||-<l> u : tNat | rNat ] ->
+  [Γ ||-<l> u' : tNat | rNat ] ->
+  [Γ ||-<l> t ≅ t' : arr tNat tNat | rNatNat ] ->
+  [Γ ||-<l> u ≅ u' : tNat | rNat ] ->
+  [Γ ||-<l> run model : arr tNat (arr tNat tPNat) | SimpleArr.ArrRedTy rNat (SimpleArr.ArrRedTy rNat rNatNat)] ->
+  [Γ ||-<l> tReflect t u ≅ tReflect t' u' : tTotal t u | rTotal ].
+Proof.
+intros * rt rt' ru ru' rtt' ruu' rrun.
+pose (rTotal' := normRedΣ0 (Induction.invLRΣ rTotal)); refold.
+fold (tTotal t u) in rTotal'.
+eapply LRTmEqIrrelevant' with (lrA := LRSig' rTotal'); [reflexivity|].
+assert (Hnft := rtt'); apply escapeEqTerm, snty_nf in Hnft.
+assert (Hnfu := ruu'); apply escapeEqTerm, snty_nf in Hnfu.
+destruct Hnft as (t₀&t'₀&[]&[]&?&?&?).
+destruct Hnfu as (u₀&u'₀&[]&[]&?&?&?).
+remember (is_closedn 0 t₀) as ct eqn:Hct; symmetry in Hct.
+assert (Hct' : is_closedn 0 t'₀ = ct).
+{ erewrite eqnf_is_closedn; [tea|now apply Symmetric_eqnf]. }
+remember (is_closedn 0 u₀) as cu eqn:Hcu; symmetry in Hcu.
+assert (Hcu' : is_closedn 0 u'₀ = cu).
+{ erewrite eqnf_is_closedn; [tea|now apply Symmetric_eqnf]. }
+remember (andb ct cu) as cb eqn:Hcb; symmetry in Hcb; destruct cb.
++ destruct ct; [|cbn in Hcb; congruence].
+  destruct cu; [|cbn in Hcb; congruence].
+  assert (∑ n₀, u₀ = qNat n₀) as [n₀]; [|subst].
+  { eapply dnf_closed_qNat; [apply ru| | |]; tea. }
+  assert (∑ n'₀, u'₀ = qNat n'₀) as [n'₀]; [|subst].
+  { eapply dnf_closed_qNat; [apply ru'| | |]; tea. }
+  clear Hcu Hcu' Hcb.
+  eapply red_redtm_exp.
+  - admit.
+  - admit.
+  - admit.
++ eapply neuTermEqRed.
+  - eapply redtm_reflect; tea.
+    all: now eapply escapeTerm.
+  - admit.
+  - admit.
+  - admit.
+  - eapply convneu_reflect.
+Admitted.
+
+Lemma ReflectRed : forall Γ l t u (rΓ : [|- Γ])
+  (rNat := natRed rΓ) (rNatNat := SimpleArr.ArrRedTy rNat rNat)
+  (rTotal : [Γ ||-<l> tTotal t u]),
+  [Γ ||-<l> t : arr tNat tNat | rNatNat] ->
+  [Γ ||-<l> u : tNat | rNat] ->
+  [Γ ||-<l> run model : arr tNat (arr tNat tPNat) | SimpleArr.ArrRedTy rNat (SimpleArr.ArrRedTy rNat rNatNat)] ->
+  [Γ ||-<l> tReflect t u : tTotal t u | rTotal].
+Proof.
+intros.
+eapply LRTmEqRed_l, ReflectRedEq; tea.
++ now eapply reflLRTmEq.
++ now eapply reflLRTmEq.
+Qed.
+
+End ReflectValid.
+
+Section ReflectValid.
+
+Context `{GenericTypingProperties}.
+Context {SN : SNTypingProperties ta _ _ _ _ _}.
+
+Lemma TyCumValid@{u i j k l u' i' j' k' l'} l Γ (vΓ : VPack@{u} Γ) A :
+typeValidity@{u i j k l} Γ vΓ l A -> typeValidity@{u' i' j' k' l'} Γ vΓ l A.
+Proof.
+intros [ty eq]; unshelve econstructor.
++ intros.
+  now eapply LRCumulative, ty.
++ intros.
+  now eapply LRTyEqIrrelevantCum, eq.
+Qed.
+
+Context {Γ l t u} (vΓ : [||-v Γ])
+  (vNat := natValid (l := l) vΓ)
+  (vArr := simpleArrValid vΓ vNat vNat)
+  (vRun := simpleArrValid vΓ vNat (simpleArrValid vΓ vNat vArr))
+  (vrun : [ Γ ||-v< l > run model : arr tNat (arr tNat tPNat) | vΓ | vRun ])
+  (vt : [ Γ ||-v< l > t : arr tNat tNat | vΓ | vArr ])
+  (vu : [ Γ ||-v< l > u : tNat | vΓ | vNat ])
+.
+
+Definition totalValid : [Γ ||-v< one > tTotal t u | vΓ].
+Proof.
+intros; unfold tTotal.
+unshelve eapply SigValid; [apply natValid|].
+apply TyCumValid.
+apply (evalValid (l := l)).
++ rewrite <- (run_ren _ ↑).
+  change (tApp (tApp (run model)⟨↑⟩ (tQuote t⟨↑⟩)) u⟨↑⟩) with
+    (tApp (tApp (run model) (tQuote t)) u)⟨↑⟩.
+  change tPNat with tPNat⟨↑⟩.
+  rewrite <- !(wk1_ren_on Γ tNat).
+  eapply irrelevanceTm', wk1ValidTm; [eapply wk1_ren_on|].
+  eapply (simple_appValid (F := tNat)); [eapply  (simple_appValid (F := tNat))|].
+  - apply vrun.
+  - apply QuoteValid; tea.
+  - tea.
++ change tNat with (tNat⟨@wk1 Γ tNat⟩) at 2.
+  unshelve eapply irrelevanceTm, var0Valid; tea.
++ rewrite <- (wk1_ren_on Γ tNat).
+  change tNat with (tNat⟨@wk1 Γ tNat⟩) at 5.
+  unshelve eapply irrelevanceTm, wk1ValidTm; tea.
+  eapply (simple_appValid (F := tNat)); tea.
+Unshelve. all: tea.
+apply simpleArrValid; tea.
+Qed.
+
+Lemma ReflectValid : [ Γ ||-v< one > tReflect t u : tTotal t u | vΓ | totalValid ].
+Proof.
+split; cbn.
+- intros Δ σ vΔ vσ; instValid vσ.
+  assert (Rtotal : [Δ ||-< one > tTotal t[σ] u[σ]]).
+  { rewrite <- tTotal_subst; eapply (validTy totalValid vΔ vσ). }
+  unshelve irrelevance0; try exact Rtotal; [now rewrite tTotal_subst|].
+  unshelve eapply ReflectRed; tea.
+  + irrelevance0; [reflexivity|]; unshelve eapply vt; tea.
+  + rewrite <- (run_subst σ); irrelevance0; [reflexivity|]; apply Rvrun.
+- intros Δ σ σ' vΔ vσ vσ' vσσ'.
+  assert (Rtotal : [Δ ||-< one > tTotal t[σ] u[σ]]).
+  { rewrite <- tTotal_subst; eapply (validTy totalValid vΔ vσ). }
+  unshelve irrelevance0; try exact Rtotal; [now rewrite tTotal_subst|].
+  eapply ReflectRedEq.
+  + irrelevance0; [reflexivity|]; unshelve eapply vt; tea.
+  + irrelevance0; [reflexivity|]; unshelve eapply vt; tea.
+  + irrelevance0; [reflexivity|]; unshelve eapply vu; tea.
+  + irrelevance0; [reflexivity|]; unshelve eapply vu; tea.
+  + irrelevance0; [reflexivity|]; unshelve eapply vt; tea.
+  + irrelevance0; [reflexivity|]; unshelve eapply vu; tea.
+  + rewrite <- (run_subst σ); irrelevance0; [reflexivity|]; apply vrun.
+  Unshelve. all: tea.
+Qed.
+
+Lemma ReflectEvalValid :
+  dnf t -> closed0 t -> dnf u -> closed0 u ->
+  [ Γ ||-v< one > tReflect t u ≅ tZero : tTotal t u | vΓ | totalValid ].
+Proof.
+Admitted.
+
+End ReflectValid.
+
+Section ReflectCongValid.
+
+Context `{GenericTypingProperties}.
+
+Context {SN : SNTypingProperties ta _ _ _ _ _}.
+
+Context {Γ l t t' u u'} (vΓ : [||-v Γ])
+  (vNat := natValid (l := l) vΓ)
+  (vArr := simpleArrValid vΓ vNat vNat)
+  (vRun := simpleArrValid vΓ vNat (simpleArrValid vΓ vNat vArr))
+  (vrun : [ Γ ||-v< l > run model : arr tNat (arr tNat tPNat) | vΓ | vRun ])
+  (vt : [ Γ ||-v< l > t : arr tNat tNat | vΓ | vArr ])
+  (vt' : [ Γ ||-v< l > t' : arr tNat tNat | vΓ | vArr ])
+  (vu : [ Γ ||-v< l > u : tNat | vΓ | vNat ])
+  (vu' : [ Γ ||-v< l > u' : tNat | vΓ | vNat ])
+.
+
+Lemma totalCongValid :
+  [Γ ||-v<l> t ≅ t' : arr tNat tNat | vΓ | vArr] ->
+  [Γ ||-v<l> u ≅ u' : tNat | vΓ | vNat ] ->
+  [Γ ||-v<one> tTotal t u ≅ tTotal t' u' | vΓ | totalValid _ vrun vt vu ].
+Proof.
+intros; unfold tTotal.
+eapply irrelevanceTyEq, SigCong; [|apply natconvValid|].
+Admitted.
+
+Lemma ReflectCongValid :
+  [Γ ||-v<l> t ≅ t' : arr tNat tNat | vΓ | vArr] ->
+  [Γ ||-v<l> u ≅ u' : tNat | vΓ | vNat ] ->
+  [Γ ||-v<one> tReflect t u ≅ tReflect t' u' : tTotal t u | vΓ | totalValid _ vrun vt vu ].
+Proof.
+Admitted.
+
+End ReflectCongValid.
